Dafny/BloodInventory.dfy
@@ -2,42 +2,41 @@ include "Blood.dfy"
 class BloodInventory
 {
     var bloodInventory: array<Blood>;
-    var bloodInventoryCover: array<string>;
     var threshold: int;
     var alert: bool;
 
     predicate Valid()
     reads this
-    requires bloodInventoryCover != null
+    requires bloodInventory != null
     {
         alert ==> (threshold >= CountByBloodType("A+")) 
     } 
 
-    // function CountByBloodType(bloodType:string): int
-    // requires bloodInventoryCover != null
-    // reads this
-    // ensures CountByBloodType(bloodType) == CheckIndexForBloodType(bloodType,  bloodInventoryCover.Length - 1)
-    // {
-    //     CheckIndexForBloodType(bloodType,  bloodInventoryCover.Length - 1)
-    // }
+    function CountByBloodType(bloodType:string): int
+    requires bloodInventory != null
+    reads this
+    ensures CountByBloodType(bloodType) == CheckIndexForBloodType(bloodType,  bloodInventory.Length - 1)
+    {
+        CheckIndexForBloodType(bloodType,  bloodInventory.Length - 1)
+    }
 
-    // function CheckIndexForBloodType(bloodType: string, index: int): int
-    // requires bloodInventoryCover != null
-    // requires index < bloodInventoryCover.Length
-    // reads this
-    // decreases index
-    // ensures (index < 0) ==> (CheckIndexForBloodType(bloodType, index) == 0)
-    // ensures (index >= 0 && (bloodInventoryCover[index] == bloodType)) ==> (CheckIndexForBloodType(bloodType, index) == CheckIndexForBloodType(bloodType, index - 1) + 1) 
-    // ensures (index >= 0 && (bloodInventoryCover[index] != bloodType)) ==> (CheckIndexForBloodType(bloodType, index) == CheckIndexForBloodType(bloodType, index - 1)) 
-    // {
-    //     if index < 0 
-    //     then
-    //         0
-    //     else
-    //         if bloodInventoryCover[index] == bloodType
-    //         then
-    //             CheckIndexForBloodType(bloodType, index - 1) + 1
-    //         else
-    //             CheckIndexForBloodType(bloodType, index - 1)
-    // }
+    function CheckIndexForBloodType(bloodType: string, index: int): int
+    requires bloodInventory != null
+    requires index < bloodInventory.Length
+    reads this
+    decreases index
+    ensures (index < 0) ==> (CheckIndexForBloodType(bloodType, index) == 0)
+    // ensures (index >= 0 && (bloodInventory[index].GetBloodType() == bloodType)) ==> (CheckIndexForBloodType(bloodType, index) == CheckIndexForBloodType(bloodType, index - 1) + 1) 
+    // ensures (index >= 0 && (bloodInventory[index].GetBloodType() != bloodType)) ==> (CheckIndexForBloodType(bloodType, index) == CheckIndexForBloodType(bloodType, index - 1)) 
+    {
+        if index < 0 
+        then
+            0
+        else
+            if bloodInventory[index].GetBloodType() == bloodType
+            then
+                CheckIndexForBloodType(bloodType, index - 1) + 1
+            else
+                CheckIndexForBloodType(bloodType, index - 1)
+    }
 } // end of BloodInventory class
